theories/typetranslation.v
@@ -4,8 +4,9 @@ From iris.algebra Require Import updates agree big_op.
 From esop Require Import types oneshot specification corecalculus overlap.
 From stdpp Require Import gmap coPset.
 
-Variant name_entry := Loc (l: loc) | Task (t: tid) (γ: gname).
+Variant name_entry := Loc (l: loc) | Task (t: tid).
 Definition name_map := gmap gname name_entry.
+Definition task_map := gmap gname gname.
 Variant conn_name := RET | name (ξ: gname) | var (x: string).
 Instance: EqDecision conn_name.
 Proof. solve_decision. Defined.
@@ -21,8 +22,8 @@ Proof.
 Qed.
 
 Definition conn_map := gmap conn_name val.
-Definition int_type {Σ} := val → name_map → val → iProp Σ.
-Definition int_heap {Σ} := conn_map → name_map → iProp Σ.
+Definition int_type {Σ} := val → task_map → name_map → val → iProp Σ.
+Definition int_heap {Σ} := conn_map → task_map → name_map → iProp Σ.
 
 Definition names_heap (η: types.heap): gset conn_name := of_list (name <$> (elements (names η))).
 Lemma elem_of_names_heap (d: conn_name) η:
@@ -77,25 +78,30 @@ Record task_data :=
       td_post: types.heap;
       td_alloc: gset gname;
       td_D_pre: conn_map;
+      td_M_pre: task_map;
       td_D_name: gname;
-      td_N_name: gname
+      td_M_name: gname;
+      td_N_name: gname;
     }.
 Canonical Structure task_dataC := leibnizC task_data.
 Canonical Structure conn_mapC := leibnizC conn_map.
 Canonical Structure name_mapC := leibnizC name_map.
+Canonical Structure task_mapC := leibnizC task_map.
 Class taskDataG Σ :=
-  { td_taskData_inG:> inG Σ (agreeR task_dataC);
+  { td_common_inG:> inG Σ (agreeR task_dataC);
     td_connData_inG:> inG Σ (oneshotR conn_mapC);
-    td_nameData_inG:> inG Σ (oneshotR name_mapC) }.
+    td_nameData_inG:> inG Σ (oneshotR name_mapC);
+    td_taskData_inG:> inG Σ (oneshotR task_mapC);
+  }.
 Local Open Scope I.
 
-Definition intΓ {Σ} (iτ: type → int_type) (Γ: env) (D: conn_map) (N: name_map)
+Definition intΓ {Σ} (iτ: type → int_type) (Γ: env) (D: conn_map) (M: task_map) (N: name_map)
            (σ: gmap string val): iProp Σ :=
   ⌜(∀ x: string, is_Some (Γ !! x) ↔ is_Some (σ !! x)) ∧
    (∀ x: string, is_Some (Γ !! x) → is_Some (D !! var x))⌝ ∧
   ∀ (x: string) τ v d, ⌜Γ !! x = Some τ ∧
                        σ !! x = Some v ∧
-                       D !! var x = Some d⌝ → iτ τ d N v.
+                       D !! var x = Some d⌝ → iτ τ d M N v.
 
 Definition not_new A: coPset := ⊤ ∖ of_gset A.
 Class InitialConfiguration := initial_cfg: cfg.
@@ -105,81 +111,91 @@ Class WaitPermissions :=
     wp_wait: ∀ `{wp_axiomaticIrisG Σ}, tid → (val → iProp Σ) → iProp Σ }.
 Existing Class wp_axiomaticIrisG.
 
-Definition simulation_body `{specStateG Σ, invG Σ, inG Σ heapR,InitialConfiguration}
-           iτ (iη: types.heap → int_heap) Γ e η A τ η' D D': iProp Σ :=
-  ∀ N σ, existential_triple ⊤ initial_cfg
-                            (intΓ iτ Γ D N σ ∗ iη η D N)
-                            (subst (of_val <$> σ) e)
-                            (λ v, ∃ d N',
-                                ⌜N ≡[not_new A]≡ N' ∧ D' !! RET = Some d⌝ ∧
-                                iτ τ d N' v ∗ iη η' D' N').
-
 Section TypeInterpretation.
   Context `{WaitPermissions, implStateG Σ, specStateG Σ, taskDataG Σ}.
   Context `{wp_axiomaticIrisG _ Σ,InitialConfiguration}.
   Implicit Type d : val.
   Implicit Type N: name_map.
+  Implicit Type M: task_map.
   Implicit Type x: val.
 
-  Definition int_i_bool d N x: iProp Σ := ⌜(x = Ctrue ∨ x = Cfalse) ∧ x = d⌝.
+  Definition int_i_bool d M N x: iProp Σ := ⌜(x = Ctrue ∨ x = Cfalse) ∧ x = d⌝.
   Definition int_s_bool := int_i_bool.
-  Definition int_i_unit d N x: iProp Σ := ⌜x = Cunit⌝.
+  Definition int_i_unit d M N x: iProp Σ := ⌜x = Cunit⌝.
   Definition int_s_unit := int_i_unit.
-  Definition int_i_ref (ξ: gname) d N x: iProp Σ := ⌜∃ l: loc, N!!ξ = Some (Loc l) ∧ x = Cloc l⌝.
+  Definition int_i_ref (ξ: gname) d M N x: iProp Σ := ⌜∃ l: loc, N!!ξ = Some (Loc l) ∧ x = Cloc l⌝.
   Definition int_s_ref := int_i_ref.
-  Definition int_s_promise ξ d N x: iProp Σ := ⌜∃ t γ, N!!ξ = Some (Task t γ) ∧ x = Ctid t⌝.
+  Definition int_s_promise ξ A (τ: type) d M N x: iProp Σ :=
+    ∃ γ (T: task_dataC),
+      own γ (to_agree T) ∗ 
+          ⌜∃ t, N!!ξ = Some (Task t) ∧ M!!ξ = Some γ ∧ x = Ctid t ∧
+                td_M_pre T ≡[names τ ∖ A]≡ M⌝.
 
   (** We build the implementation interpretation of promise in stages. *)
   (** Access to the task data. *)
-  Definition ip_data γ U (D': conn_map) (N': name_map) :=
-    own γ (to_agree U) ∗ own (td_D_name U) (agreed D') ∗ own (td_N_name U) (agreed N').
+  Definition ip_data γ U (D': conn_map) (M': task_map) (N': name_map) :=
+    own γ (to_agree U) ∗ own (td_D_name U) (agreed D') ∗ own (td_N_name U) (agreed N') ∗
+        own (td_M_name U) (agreed M').
+  
   (** The easy parts: name map and implementation interpretation. *)
-  Definition ip_impl (A: gset gname) (τ: type) (τi: @int_type Σ) (D': conn_map) N' N y :=
-    ∃ d, ⌜D' !! RET = Some d ∧ N' ≡[ names τ ∖ A ]≡ N⌝ ∗ τi d N' y.
-  Definition ip_sim iτs iηs τ U D' :=
-    simulation_body iτs iηs
-                    (td_env U) (td_expr U) (td_pre U) (td_alloc U) τ (td_post U) (td_D_pre U) D'.
+  Definition ip_impl (A: gset gname) (τ: type) (τi: @int_type Σ) (D': conn_map) M' N' M N y :=
+    ∃ d, ⌜D' !! RET = Some d ∧ N' ≡[ names τ ∖ A ]≡ N ∧ M' ≡[ names τ ∖ A]≡ M⌝ ∗ τi d M' N' y.
+  Definition ip_sim iτs iηs A (τ: type) U D' M': iProp Σ :=
+    ∀ N N' σ (eqN: N ≡[(names τ ∪ names (td_post U)) ∖ td_alloc U]≡ N') (eqA: td_alloc U = A),
+      existential_triple ⊤ initial_cfg
+                         (intΓ iτs (td_env U) (td_D_pre U) (td_M_pre U) N' σ ∗
+                               iηs (td_pre U) (td_D_pre U) (td_M_pre U) N')
+                         (subst (of_val <$> σ) (td_expr U))
+                         (λ v, ∃ d N'', ⌜N ≡[not_new (td_alloc U)]≡ N'' ∧ D' !! RET = Some d⌝ ∧
+                                        iτs τ d M' N'' v ∗ iηs (td_post U) D' M' N'').
   (** Put together the inner pieces of the interpretation of promises... *)
   Definition promiseN := nroot .@ "promise".
-  Definition int_i_promise_body iτs iηs N A τ τi γ v :=
-    ∃ U D' N',
-      ip_data γ U D' N' ∗ ip_impl A τ τi D' N' N v ∗ □ip_sim iτs iηs τ U D'.
-  Definition int_i_promise iτs iηs ξ A τ τi d N x :=
-    ∃ t γ, ⌜N !! ξ = Some (Task t γ) ∧ x = Ctid t⌝ ∧
-           inv promiseN (wp_wait t (int_i_promise_body iτs iηs (delete ξ N) A τ τi γ)).
+  Definition int_i_promise_body iτs iηs M N A τ τi γ v :=
+    ∃ U D' M' N',
+      ip_data γ U D' M' N' ∗ ip_impl A τ τi D' M' N' M N v ∗ □ip_sim iτs iηs A τ U D' M'.
+  Definition int_i_promise iτs iηs ξ A τ τi d M N x :=
+    ∃ t γ, ⌜N !! ξ = Some (Task t) ∧ M !! ξ = Some γ ∧ x = Ctid t⌝ ∧
+           inv promiseN (wp_wait t (int_i_promise_body iτs iηs (delete ξ M) (delete ξ N) A τ τi γ)).
 End TypeInterpretation.
 
 Section HeapInterpretation.
   Context `{WaitPermissions, implStateG Σ, specStateG Σ, wp_axiomaticIrisG _ Σ, taskDataG Σ}.
   Implicit Type N : name_map.
+  Implicit Type M : task_map.
   Implicit Type D : conn_map.
   Local Open Scope I.
 
-  Definition int_i_emp D N: iProp Σ := True.
+  Definition int_i_emp D M N: iProp Σ := True.
   Definition int_s_emp := int_i_emp.
-  Definition int_i_star (iη iη': int_heap) D N: iProp Σ := iη D N ∗ iη' D N.
+  Definition int_i_star (iη iη': int_heap) D M N: iProp Σ := iη D M N ∗ iη' D M N.
   Definition int_s_star := int_i_star.
-  Definition int_i_pt ξ (iτ: int_type) D N: iProp Σ :=
-    ∃ l d v, ⌜N!!ξ = Some (Loc l) ∧ D!!name ξ = Some d⌝ ∗ mapstoI l v 1%Qp ∗ iτ d N v.
-  Definition int_s_pt ξ (iτ: int_type) D N: iProp Σ :=
-    ∃ l d v, ⌜N!!ξ = Some (Loc l) ∧ D!!name ξ = Some d⌝ ∗ mapstoS l v 1%Qp ∗ iτ d N v.
-  Definition int_i_wait_body γ (η: types.heap) (iη: int_heap) A N :=
-    ∃ U D' N', ip_data γ U D' N' ∗ ⌜N ≡[ names η ∖ A]≡ N'⌝ ∗ iη D' N'.
-  Definition int_i_wait ξ A η (iη: int_heap) D N: iProp Σ :=
-    ∃ t γ, ⌜N!!ξ = Some (Task t γ)⌝ ∗ wp_wait t (λ _, int_i_wait_body γ η iη A (delete ξ N)).
+  Definition int_i_pt ξ (iτ: int_type) D M N: iProp Σ :=
+    ∃ l d v, ⌜N!!ξ = Some (Loc l) ∧ D!!name ξ = Some d⌝ ∗ mapstoI l v 1%Qp ∗ iτ d M N v.
+  Definition int_s_pt ξ (iτ: int_type) D M N: iProp Σ :=
+    ∃ l d v, ⌜N!!ξ = Some (Loc l) ∧ D!!name ξ = Some d⌝ ∗ mapstoS l v 1%Qp ∗ iτ d M N v.
+  Definition int_i_wait_body γ (η: types.heap) (iη: int_heap) A M N :=
+    ∃ U D' N' M', ip_data γ U D' M' N' ∗ ⌜N ≡[ names η ∖ A]≡ N' ∧ M ≡[names η ∖ A]≡ M'⌝ ∗ iη D' M' N'.
+  Definition int_i_wait ξ A η (iη: int_heap) D M N: iProp Σ :=
+    ∃ t γ, ⌜N!!ξ = Some (Task t) ∧ M!!ξ = Some γ⌝ ∗
+                                               wp_wait t (λ _, int_i_wait_body γ η iη A (delete ξ M)
+                                                                               (delete ξ N)).
   (* Use the lower-level interpretations here *)
-  Definition int_s_wait_pre iτs' (iηs': types.heap → int_heap) U N' σ: iProp Σ :=
-    intΓ iτs' (td_env U) (td_D_pre U) N' σ ∗ iηs' (td_pre U) (td_D_pre U) N'.
-  Definition int_s_wait iτs' iηs' ξ A η D N :=
-    ∃ t γ U N' σ,
-      ⌜N!!ξ = Some (Task t γ) ∧ td_post U = η ∧ N' ≡[names η ∖ A]≡ N⌝ ∧
-      t ⤇ run: (subst (of_val <$> σ) (td_expr U)) ∗ int_s_wait_pre iτs' iηs' U N' σ.
+  Definition int_s_wait_pre iτs' (iηs': types.heap → int_heap) U σ: iProp Σ :=
+    ∃ N, intΓ iτs' (td_env U) (td_D_pre U) (td_M_pre U) N σ ∗
+              iηs' (td_pre U) (td_D_pre U) (td_M_pre U) N.
+  Definition int_s_wait iτs' iηs' ξ A η D M N :=
+    ∃ t γ U σ,
+      ⌜N!!ξ = Some (Task t) ∧ M!!ξ = Some γ ∧
+      td_post U = η ∧ td_alloc U = A ∧
+      td_M_pre U ≡[names η ∖ A]≡ M⌝ ∧ own γ (to_agree U) ∗
+      t ⤇ run: (subst (of_val <$> σ) (td_expr U)) ∗ int_s_wait_pre iτs' iηs' U σ.
 End HeapInterpretation.
 
 Section Interpretations.
   Context `{WaitPermissions, implStateG Σ, specStateG Σ, wp_axiomaticIrisG _ Σ, taskDataG Σ}.
   Context `{InitialConfiguration, ∀ t, Proper (pointwise_relation _ (≡) ==> (≡)) (wp_wait t)}.
   Implicit Type N: name_map.
+  Implicit Type M: task_map.
   Implicit Type D: conn_map.
   Implicit Type x: val.
   Implicit Type d: val.
@@ -190,7 +206,7 @@ Section Interpretations.
     | tbool => int_s_bool
     | tunit => int_s_unit
     | tref ξ => int_s_ref ξ
-    | ttask ξ A τ => int_s_promise ξ
+    | ttask ξ A τ => int_s_promise ξ A τ
     end.
   Fixpoint int_s_heap_approx iη η: @int_heap Σ :=
     match η with
@@ -201,11 +217,11 @@ Section Interpretations.
     end.
   Fixpoint int_s_heap_rec n η :=
     int_s_heap_approx (match n with
-                       | O => λ _ _ _, False%I
+                       | O => λ _ _ _ _, False%I
                        | S n => int_s_heap_rec n
                        end)
                       η.
-  Definition int_s_heap η: @int_heap Σ := λ D N, ∃ n, int_s_heap_rec n η D N.
+  Definition int_s_heap η: @int_heap Σ := λ D M N, ∃ n, int_s_heap_rec n η D M N.
 
   Fixpoint int_i_type τ: @int_type Σ :=
     match τ with
@@ -226,42 +242,46 @@ Section Interpretations.
   Definition int_i_env := intΓ int_i_type.
   
   (** Basic properties of interpretation *)
-  Global Instance int_s_type_persistent τ d N v:  PersistentP (int_s_type τ d N v).
+  Global Instance int_s_type_persistent τ d M N v:  PersistentP (int_s_type τ d M N v).
   Proof. destruct τ; apply _. Qed.
-  Global Instance int_i_type_persistent τ d N v:  PersistentP (int_i_type τ d N v).
+  Global Instance int_i_type_persistent τ d M N v:  PersistentP (int_i_type τ d M N v).
   Proof. destruct τ; apply _. Qed.
-  Global Instance int_s_env_persistent Γ D N σ: PersistentP (int_s_env Γ D N σ).
+  Global Instance int_s_env_persistent Γ D M N σ: PersistentP (int_s_env Γ D M N σ).
   Proof. apply _. Qed.
-  Global Instance int_i_env_persistent Γ D N σ: PersistentP (int_i_env Γ D N σ).
+  Global Instance int_i_env_persistent Γ D M N σ: PersistentP (int_i_env Γ D M N σ).
   Proof. apply _. Qed.
 
   Global Instance int_s_type_local τ:
-    Proper ((=) ==> overlap (names τ) ==> (=) ==> (⊣⊢)) (int_s_type τ).
+    Proper ((=) ==> overlap (names τ) ==> overlap (names τ) ==> (=) ==> (⊣⊢)) (int_s_type τ).
   Proof.
-    induction τ; intros d ? <- N N' eqN x ? <-; cbn; try done.
+    induction τ; intros d ? <- M M' eqM N N' eqN x ? <-; cbn; try done.
     - rewrite /int_s_ref /int_i_ref.
       rewrite eqN; first done.
       cbn; set_solver.
     - rewrite /int_s_promise.
-      rewrite eqN; first done.
-      cbn -[union]; set_solver.
+      f_equiv; intro γ.
+      f_equiv; intro T.
+      do 3 f_equiv; intro t.
+      rewrite (eqM ξ) ?(eqN ξ).
+      2,3: by apply elem_of_union_l, elem_of_singleton.
+      do 3 f_equiv.
+      apply (overlap_iff (names (ttask ξ A τ))); last done.
+      apply union_subseteq_r.
   Qed.
 
   Global Instance int_i_type_local τ:
-    Proper ((=) ==> overlap (names τ) ==> (=) ==> (⊣⊢)) (int_i_type τ).
+    Proper ((=) ==> overlap (names τ) ==> overlap (names τ) ==> (=) ==> (⊣⊢)) (int_i_type τ).
   Proof.
-    induction τ; intros d ? <- N N' eqN x ? <-; cbn; try done.
+    induction τ; intros d ? <- M M' eqM N N' eqN x ? <-; cbn; try done.
     - rewrite /int_i_ref eqN; first done.
       cbn; set_solver.
     - rewrite /int_i_promise /int_i_promise_body /ip_impl.
       rewrite (eqN ξ); last set_solver.
-      do 21 f_equiv.
-      apply (overlap_iff ((names (ttask ξ A τ)))).
-      + apply union_subseteq_r.
-      + intros ξ' inξ'.
-        destruct (decide (ξ = ξ')) as [<-|neq].
-        * by rewrite !lookup_delete.
-        * rewrite !lookup_delete_ne; auto.
+      rewrite (eqM ξ); last set_solver.
+      do 24 f_equiv.
+      all: apply (overlap_iff ((names (ttask ξ A τ)))).
+      1,3: apply union_subseteq_r.
+      all: by apply overlap_delete_proper.
   Qed.
 
   Lemma names_heap_star η η': (names_heap (η ⊗ η') ≡ names_heap η ∪ names_heap η')%C.
@@ -278,95 +298,106 @@ Section Interpretations.
   
   Lemma int_s_heap_approx_local
         iη (iη_proper: ∀ (η: types.heap),
-               Proper (overlap (names_heap η) ==> overlap (names η) ==> (⊣⊢)) (iη η)) η:
-    Proper (overlap (names_heap η) ==> overlap (names η) ==> (⊣⊢)) (int_s_heap_approx iη η).
+               Proper (overlap (names_heap η) ==> overlap (names η) ==> overlap (names η) ==> (⊣⊢))
+                      (iη η)) η:
+    Proper (overlap (names_heap η) ==> overlap (names η) ==> overlap (names η) ==> (⊣⊢))
+           (int_s_heap_approx iη η).
   Proof.
-    induction η; intros D D' eqD N N' eqN; cbn.
+    induction η; intros D D' eqD M M' eqM N N' eqN; cbn.
     - done.
     - rewrite /int_s_star /int_i_star.
       f_equiv; [apply IHη1|apply IHη2].
       all: eapply overlap_mono; eauto.
       all: cbn.
-      1,3: rewrite names_heap_star.
-      all: clear; set_solver.
+      1,4: rewrite names_heap_star.
+      1,3,4: apply union_subseteq_l.
+      all: apply union_subseteq_r.
     - rewrite /int_s_pt.
-      setoid_rewrite (eqN ξ); last by set_solver.
+      setoid_rewrite (eqN ξ); last (rewrite /= elem_of_union elem_of_singleton; auto).
       rewrite eqD; cycle 1.
-      { rewrite /names_heap elem_of_of_list elem_of_list_fmap.
+      { rewrite elem_of_names_heap.
         exists ξ; split; auto.
-        rewrite elem_of_elements; set_solver. }
-      enough (∀ d v, int_s_type τ d N v ⊣⊢ int_s_type τ d N' v) as eqint.
+        rewrite /= elem_of_union elem_of_singleton; auto. }
+      enough (∀ d v, int_s_type τ d M N v ⊣⊢ int_s_type τ d M' N' v) as eqint.
       { by setoid_rewrite eqint. }
       intros; apply int_s_type_local; auto.
-      eapply overlap_mono; eauto.
-      set_solver.
+      all: eapply overlap_mono; eauto.
+      all: intros ??; apply elem_of_union; auto.
     - rewrite /int_s_wait /=.
       do 10 f_equiv.
       rewrite (eqN ξ); last set_solver.
+      rewrite (eqM ξ); last set_solver.
       do 4 f_equiv.
-      apply (overlap_iff ((names (hwait ξ A η)))); eauto.
-      apply union_subseteq_r.
+      all: eapply overlap_iff; last done.
+      all: apply union_subseteq_r.
   Qed.
 
   Lemma int_s_heap_rec_local n: ∀ η,
-      Proper (overlap (names_heap η) ==> overlap (names η) ==> (⊣⊢)) (int_s_heap_rec n η).
+      Proper (overlap (names_heap η) ==> overlap (names η) ==> overlap (names η) ==> (⊣⊢))
+             (int_s_heap_rec n η).
   Proof.
     induction n as [|n IH]; intros; cbn; apply int_s_heap_approx_local; auto.
     solve_proper.
   Qed.
 
   Lemma int_s_heap_local η:
-    Proper (overlap (names_heap η) ==> overlap (names η) ==> (⊣⊢)) (int_s_heap η).
+    Proper (overlap (names_heap η) ==> overlap (names η) ==> overlap (names η) ==> (⊣⊢))
+           (int_s_heap η).
   Proof.
-    intros D D' eqD N N' eqN.
+    intros D D' M M' eqM eqD N N' eqN.
     rewrite /int_s_heap.
     f_equiv; intro n.
     apply int_s_heap_rec_local; done.
   Qed.
   
   Lemma int_i_heap_local η:
-    Proper (overlap (names_heap η) ==> overlap (names η) ==> (⊣⊢)) (int_i_heap η).
+    Proper (overlap (names_heap η) ==> overlap (names η) ==> overlap (names η) ==> (⊣⊢))
+           (int_i_heap η).
   Proof.
-    induction η; intros D D' eqD N N' eqN; cbn.
+    induction η; intros D D' eqD M M' eqM N N' eqN; cbn.
     - done.
     - rewrite /int_s_star /int_i_star.
       f_equiv; [apply IHη1|apply IHη2].
       all: eapply overlap_mono; eauto.
       all: cbn.
-      1,3: rewrite names_heap_star.
-      all: clear; set_solver.
+      1,4: rewrite names_heap_star.
+      1,3,4: apply union_subseteq_l.
+      all: apply union_subseteq_r.
     - rewrite /int_i_pt.
       rewrite (eqN ξ); last set_solver.
       rewrite (eqD (name ξ)).
-      2: rewrite /names_heap elem_of_of_list elem_of_list_fmap.
-      2: eexists; split; eauto.
-      2: rewrite elem_of_elements; set_solver.
+      2: rewrite elem_of_names_heap /=.
+      2: eexists _; split; auto; apply elem_of_union; rewrite elem_of_singleton; auto.
       assert (N ≡[ names τ ]≡ N') as eqN'.
       { intros ξ' inξ; apply eqN; set_solver. }
-      enough (∀ d v, int_i_type τ d N v ⊣⊢ int_i_type τ d N' v) as eqτ.
+      assert (M ≡[ names τ ]≡ M') as eqM'.
+      { intros ξ' inξ; apply eqM; set_solver. }
+      enough (∀ d v, int_i_type τ d M N v ⊣⊢ int_i_type τ d M' N' v) as eqτ.
       { by setoid_rewrite eqτ. }
       intros; by apply int_i_type_local.
     - rewrite /int_i_wait /int_i_wait_body.
       rewrite (eqN ξ); last set_solver.
-      enough (∀ N'', delete ξ N ≡[ names η ∖ A ]≡ N'' ↔
-                       delete ξ N' ≡[ names η ∖ A ]≡ N'')
-        as eqN'.
-      { by setoid_rewrite eqN'. }
-      intro.
+      rewrite (eqM ξ); last set_solver.
+      enough (∀ M'' N'', (delete ξ N ≡[ names η ∖ A ]≡ N'' ∧ delete ξ M ≡[ names η ∖ A ]≡ M'')
+                           ↔ (delete ξ N' ≡[ names η ∖ A ]≡ N'' ∧ delete ξ M' ≡[ names η ∖ A ]≡ M''))
+        as eqMN'.
+      { by setoid_rewrite eqMN'. }
+      intros.
       rewrite -!(symmetry_iff (overlap (names η ∖ A)) N'').
-      apply (overlap_iff (names (hwait ξ A η))).
-      + apply union_subseteq_r.
-      + intros ξ' inξ'.
-        destruct (decide (ξ = ξ')) as [<-|neq].
-        * by rewrite !lookup_delete.
-        * rewrite !lookup_delete_ne; auto.
+      rewrite -!(symmetry_iff (overlap (names η ∖ A)) M'').
+      f_equiv.
+      all: apply (overlap_iff (names (hwait ξ A η))).
+      1,3: apply union_subseteq_r.
+      all: by apply overlap_delete_proper.
   Qed.
 
   Lemma intΓ_local (ϕ: type → @int_type Σ)
-        (ϕ_local: ∀ τ, Proper ((=) ==> overlap (names τ) ==> (=) ==> (⊣⊢)) (ϕ τ)) Γ:
-    Proper (overlap (names_env Γ) ==> overlap (names Γ) ==> (=) ==> (⊣⊢)) (intΓ ϕ Γ).
+        (ϕ_local: ∀ τ, Proper ((=) ==> overlap (names τ) ==> overlap (names τ) ==> (=) ==> (⊣⊢))
+                              (ϕ τ)) Γ:
+    Proper (overlap (names_env Γ) ==> overlap (names Γ) ==> overlap (names Γ) ==> (=) ==> (⊣⊢))
+           (intΓ ϕ Γ).
   Proof.
-    intros D D' eqD N N' eqN σ ? <-.
+    intros D D' eqD M M' eqM N N' eqN σ ? <-.
     rewrite /intΓ.
     assert (pure_l_and: ∀ P P' (Q Q': iProp Σ) (eqP: (P ↔ P')%type) (eqQ: P → Q ⊣⊢ Q'),
                ⌜P⌝ ∧ Q ⊣⊢ ⌜P'⌝ ∧ Q').
@@ -390,53 +421,57 @@ Section Interpretations.
     rewrite (eqD (var x)); last done.
     f_equiv.
     apply ϕ_local; try done.
-    eapply overlap_mono.
-    2,3,4: done.
-    intro ξ.
-    rewrite env_elem_of_names.
-    exists x,τ; auto.
+    all: eapply overlap_mono.
+    2,3,4,6,7,8: done.
+    all: intro ξ; rewrite env_elem_of_names; exists x,τ; eauto.
   Qed.
 
   Lemma int_i_env_local Γ: 
-    Proper (overlap (names_env Γ) ==> overlap (names Γ) ==> (=) ==> (⊣⊢)) (int_i_env  Γ).
+    Proper (overlap (names_env Γ) ==> overlap (names Γ) ==> overlap (names Γ) ==> (=) ==> (⊣⊢))
+           (int_i_env  Γ).
   Proof. apply intΓ_local, int_i_type_local. Qed.
   Lemma int_s_env_local Γ: 
-    Proper (overlap (names_env Γ) ==> overlap (names Γ) ==> (=) ==> (⊣⊢)) (int_s_env  Γ).
+    Proper (overlap (names_env Γ) ==> overlap (names Γ) ==> overlap (names Γ) ==> (=) ==> (⊣⊢))
+           (int_s_env  Γ).
   Proof. apply intΓ_local, int_s_type_local. Qed.
   
-  Lemma int_s_heap_approx_mono ϕ ϕ' (mono: ∀ η D N, ϕ η D N -∗ ϕ' η D N) η:
-    ∀ D N, int_s_heap_approx ϕ η D N -∗ int_s_heap_approx ϕ' η D N.
+  Lemma int_s_heap_approx_mono ϕ ϕ' (mono: ∀ η D M N, ϕ η D M N -∗ ϕ' η D M N) η:
+    ∀ D M N, int_s_heap_approx ϕ η D M N -∗ int_s_heap_approx ϕ' η D M N.
   Proof.
     induction η; cbn.
-    - iIntros (??) "$".
-    - iIntros (D N) "[I1 I2]".
+    - iIntros (???) "$".
+    - iIntros (D M N) "[I1 I2]".
       iSplitL "I1".
       + iApply (IHη1 with "I1").
       + iApply (IHη2 with "I2").
-    - iIntros (??) "$".
-    - iIntros (D N).
+    - iIntros (???) "$".
+    - iIntros (D M N).
       rewrite /int_s_wait /int_s_wait_pre.
       iIntros "pre".
-      iDestruct "pre" as (t γ U N' σ) "[pre [move [env wait]]]".
-      iExists t,γ,U,N',σ; iFrame.
-      iApply (mono with "wait").
+      iDestruct "pre" as (t γ U σ) "[names [agree [move pre]]]".
+      iExists t,γ,U,σ; iFrame.
+      iDestruct "pre" as (N') "wait".
+      iExists N'.
+      iDestruct "wait" as "[$ ϕ]".
+      iApply (mono with "ϕ").
   Qed.
-  Lemma int_s_heap_rec_S n: ∀ η D N, int_s_heap_rec n η D N -∗ int_s_heap_rec (S n) η D N.
+  Lemma int_s_heap_rec_S n: ∀ η D M N, int_s_heap_rec n η D M N -∗ int_s_heap_rec (S n) η D M N.
   Proof.
     rewrite -Nat.add_1_r.
     induction n as [|n IH]; cbn.
-    all: iIntros (η D N) "pre"; iApply (int_s_heap_approx_mono with "pre").
-    - iIntros (???) "[]".
+    all: iIntros (η D M N) "pre"; iApply (int_s_heap_approx_mono with "pre").
+    - iIntros (????) "[]".
     - exact IH.
   Qed.
   
   Lemma int_s_heap_rec_mono n n' (len: n ≤ n'):
-    ∀ η D N, int_s_heap_rec n η D N -∗ int_s_heap_rec n' η D N.
+    ∀ η D M N, int_s_heap_rec n η D M N -∗ int_s_heap_rec n' η D M N.
   Proof.
     induction len.
-    { iIntros (???) "$". }
-    iIntros (η D N) "pre".
+    { iIntros (????) "$". }
+    iIntros (η D M N) "pre".
     iApply (int_s_heap_rec_S with "[-]").
     iApply (IHlen with "pre").
   Qed.
 End Interpretations.
+
